LambdaLab.lean
@@ -26,7 +26,7 @@ import LambdaLab.Parser.Mixfix.Parser
 import LambdaLab.Stlc.Named.Parser
 import LambdaLab.Stlc.Named.Lang
 import LambdaLab.Stlc.Named.Unification
-import LambdaLab.Stlc.Named.HM
+import LambdaLab.Stlc.Named.W
 import LambdaLab.Language.Basic
 import LambdaLab.Language.Parser
 import LambdaLab.Language.Check
